\documentclass[11pt]{article}

\begin{document}
\begin{center}
\large \textbf{Answer Key for Exercise 3.1}	
\end{center}
\bigskip

\noindent \textbf{Permutation}\smallskip \\
\noindent
\begin{tabular}{l l l l}
$1$ & (1) $P \rightarrow (Q \rightarrow R)$ & A \\
$2$ & (2) $P$ & A \\
$3$ & (3) $Q$ & A \\
$1,2$ & (4) $Q \rightarrow R$ & MPP 2,1 \\
$1,2,3$ & (4) $R$ & MPP 3,4 \\
$1,3$ & (5) $(P \rightarrow R)$ & CP 2,4 \\
$1$ & (6) $Q \rightarrow (P \rightarrow R)$ & CP 3,1 \\
\end{tabular}
\bigskip\\
\noindent \textbf{Suffixing}\smallskip \\
\begin{tabular}{l l l l}
$1$ & (1) $P \rightarrow Q$ & A \\
$2$ & (2) $Q \rightarrow R$ & A \\
$3$ & (3) $P$ & A \\
$1,3$ & (4) $Q$ & MPP 3,1 \\
$1,2,3$ & (5) $R$ & MPP 4,2 \\
$1,2$ & (6) $P \rightarrow R$ & CP 3,5 \\
$1$ & (7) $(Q \rightarrow R) \rightarrow (P \rightarrow R)$ & CP 2,6 \\
\end{tabular}
\bigskip\\
\noindent \textbf{Contraction}\smallskip \\
\begin{tabular}{l l l l}
$1$ & (1) $P \rightarrow (P \rightarrow Q)$ & A \\
$2$ & (2) $P$ & A \\
$1,2$ & (3) $P \rightarrow Q$ & MPP 2,1 \\
$1,2$ & (4) $Q$ & MPP 2,3 \\
$1$ & (5) $P \rightarrow Q$ & CP 2,4\\
\end{tabular}
\bigskip\\
\noindent \textbf{Exportation}\smallskip \\
\begin{tabular}{l l l l}
$1$ & (1) $P \rightarrow (Q \rightarrow R)$ & A \\
$2$ & (2) $P \wedge Q$ & A \\
$2$ & (3) $P$ & $\wedge$E  \\
$2$ & (4) $Q$ & $\wedge$E  \\
$1,2$ & (5) $Q \rightarrow R$ & MPP 3,1 \\
$1,2$ & (6) $R$ & MPP 4,5 \\
$1$ & (7) $(P \wedge Q) \rightarrow R$ & CP 2,6 \\
\end{tabular}
\newpage
\noindent \textbf{Strengthening}\smallskip \\\begin{tabular}{l l l l}
$1$ & (1) $(P \vee Q) \rightarrow R$ & A \\
$2$ & (2) $P$ & A \\
$2$ & (3) $P \vee Q$ & $\wedge$I \\
$1,2$ & (4) $R$ & MPP 3,1 \\
$1$ & (5) $P \rightarrow R$ & CP 2,4 \\
\end{tabular}
\bigskip\\
\noindent \textbf{DeMorgan's Rule}\smallskip \\
\begin{tabular}{l l l l}
$1$ & (1) $\neg(P \vee Q)$ & A \\
$2$ & (2) $P$ & A \\
$2$ & (3) $P \vee Q$ & $\vee$I \\
$$ & (4) $P \rightarrow (P \vee Q)$ & CP 2,3 \\
$1$ & (5) $\neg P$ & MTT 1,4 \\
$6$ & (6) $Q$ & A \\
$6$ & (7) $P \vee Q$ & $\vee$I \\
$$ & (8) $Q \rightarrow (P \vee Q)$ & CP 6,7 \\
$1$ & (9) $\neg Q$ & MTT 1,8 \\
$1$ & (10) $\neg P \wedge \neg Q$ & $\wedge$I 5,9 \\
\end{tabular}

\bigskip \bigskip 


\noindent To show that $P\to \neg P\vdash \neg P$:
\begin{enumerate}
\item By MPP and CP, $P\vdash ((P\to \neg P)\to \neg P)$
\item By contraposition, $P\vdash P\to \neg (P\to \neg P)$
\item By contraction, $\vdash P\to \neg (P\to \neg P)$
\item By contraposition, $\vdash (P\to \neg P)\to \neg P$
\item By MPP, $P\to\neg P\vdash \neg P$
\end{enumerate}


\end{document}


%%% Local Variables:
%%% mode: latex
%%% TeX-master: t
%%% End:







